@prefix owl: <http://www.w3.org/2002/07/owl#> .
@prefix dc11: <http://purl.org/dc/elements/1.1/> .
@prefix xsd: <http://www.w3.org/2001/XMLSchema#> .
@prefix rdfs: <http://www.w3.org/2000/01/rdf-schema#> .
@prefix foaf: <http://xmlns.com/foaf/0.1/> .
@prefix rdf: <http://www.w3.org/1999/02/22-rdf-syntax-ns#> .
@prefix lexinfo: <http://www.lexinfo.net/ontology/2.0/lexinfo#> .
@prefix twtr: <http://example.org/> .

twtr:
  a owl:Ontology ;
  dc11:date "$Date: 2017-04-21 23:18:26 $" ;
  dc11:creator "Ralph Offinger"^^xsd:string ;
  dc11:description "The Twitter (TWTR) RDF vocabulary, described using W3C RDF Schema." ;
  dc11:title "TWTR (Twitter) vocabulary" .

twtr:Tweet
  rdf:type owl:Class , rdfs:Class ;
  rdfs:isDefinedBy twtr: ;
  rdfs:comment "A tweet is a text message limited to 140 characters in length, that is broadcast and readable by anyone who accesses Twitter." ;
  rdfs:label "Tweet" .

twtr:TwitterAccount
  rdf:type owl:Class , rdfs:Class ;
  rdfs:isDefinedBy twtr: ;
  rdfs:comment "An account on the social networking site Twitter" ;
  rdfs:label "Twitter Account" .

twtr:TweetSubject
  rdf:type owl:Class , rdfs:Class ;
  rdfs:comment "The relation between a phrase and a verb in a tweet, that represents the person or thing that performs the action or about which something is stated." ;
  rdfs:isDefinedBy twtr: ;
  rdfs:label "Tweet Subject" .

twtr:TweetObject
  rdf:type owl:Class , rdfs:Class ;
  rdfs:comment "The relation between a phrase and a verb in a tweet, in which the relation is central to the verb." ;
  rdfs:isDefinedBy twtr: ;
  rdfs:label "Tweet Object" .

twtr:followerCount
  rdf:type    rdf:Property , owl:DatatypeProperty ;
  rdfs:comment "Amount of users who have subscribed to a Twitter Account." ;
  rdfs:isDefinedBy twtr: ;
  rdfs:label "follower count" ;
  rdfs:domain twtr:TwitterAccount ;
  rdfs:range xsd:integer .

twtr:userID
  rdf:type    rdf:Property , owl:DatatypeProperty ;
  rdfs:comment "A Twitter Account ID." ;
  rdfs:isDefinedBy twtr: ;
  rdfs:label "user ID" ;
  rdfs:domain twtr:TwitterAccount ;
  rdfs:range rdfs:Literal .

twtr:userName
  rdf:type    rdf:Property , owl:DatatypeProperty ;
  rdfs:comment "A short informal nickname characterising a Twitter Account." ;
  rdfs:isDefinedBy twtr: ;
  rdfs:label "username" ;
  rdfs:domain twtr:TwitterAccount ;
  rdfs:range rdfs:Literal .

twtr:userDescription
  rdf:type    rdf:Property , owl:DatatypeProperty ;
  rdfs:comment "A short personal description of a Twitter Account." ;
  rdfs:isDefinedBy twtr: ;
  rdfs:label "user description" ;
  rdfs:domain twtr:TwitterAccount ;
  rdfs:range rdfs:Literal .

twtr:tweetText
  rdf:type    rdf:Property , owl:DatatypeProperty ;
  rdfs:comment "A status message within Twitter." ;
  rdfs:isDefinedBy twtr: ;
  rdfs:label "Tweet Text" ;
  rdfs:domain twtr:Tweet ;
  rdfs:range rdfs:Literal .

twtr:tweetID
  rdf:type    rdf:Property , owl:DatatypeProperty ;
  rdfs:comment "A Tweet ID." ;
  rdfs:isDefinedBy twtr: ;
  rdfs:label "tweet ID" ;
  rdfs:domain twtr:Tweet ;
  rdfs:range xsd:integer .

twtr:tweeted
  rdf:type    rdf:Property , owl:ObjectProperty ;
  rdfs:comment "A Tweet gets tweeted from a TwitterAccount." ;
  rdfs:domain twtr:TwitterAccount ;
  rdfs:isDefinedBy twtr: ;
  rdfs:label "tweeted" ;
  rdfs:range twtr:Tweet .

twtr:mentions
  rdf:type    rdf:Property , owl:ObjectProperty ;
  rdfs:comment "A Tweet might mention a subject." ;
  rdfs:domain twtr:Tweet ;
  rdfs:isDefinedBy twtr: ;
  rdfs:label "mentions" ;
  rdfs:range twtr:TweetSubject .

twtr:verb
  rdf:type    rdf:Property , owl:ObjectProperty ;
  rdfs:comment "A verb signals an action, an occurrence, or a state of being." ;
  rdfs:domain twtr:TweetSubject ;
  rdfs:isDefinedBy twtr: ;
  rdfs:label "verb" ;
  rdfs:range twtr:TweetObject .